verified/smcapi.s.dfy
@@ -408,7 +408,7 @@ predicate smcNonvolatileRegInvariant(s:state, s':state)
 }
 
 /* Overall invariant across SMC handler state */
-predicate smchandlerInvariant(s:state, s':state)
+predicate smchandlerInvariant(s:state, s':state, entry:bool)
     requires ValidState(s) && ValidState(s')
 {
     reveal_ValidRegState();
@@ -420,16 +420,24 @@ predicate smchandlerInvariant(s:state, s':state)
         // return to a non-monitor mode (so we leave secure world)
         && decode_mode(psr_mask_mode(s.sregs[spsr(Monitor)])) != Monitor
         // most banked regs are preserved -- carve-outs for IRQ/FIQ injection 
-        && (forall m | m !in {Monitor, IRQ, FIQ} ::
-            (m != User ==> s.sregs[spsr(m)] == s'.sregs[spsr(m)])
-            && s.regs[LR(m)] == s'.regs[LR(m)])
         && (forall m :: s.regs[SP(m)] == s'.regs[SP(m)])
+        && (if entry then 
+            (forall m | m !in {Monitor, IRQ, FIQ} ::
+                (m != User ==> s.sregs[spsr(m)] == s'.sregs[spsr(m)])
+                && s.regs[LR(m)] == s'.regs[LR(m)])
+        else
+            InsecureMemInvariant(s, s')
+            && (forall m :: s.regs[LR(m)] == s'.regs[LR(m)])
+            && (forall m | m != User :: s.sregs[spsr(m)] == s.sregs[spsr(m)]))
 }
 
 predicate smchandler(s: state, pageDbIn: PageDb, s':state, pageDbOut: PageDb)
     requires ValidState(s) && validPageDb(pageDbIn) && SaneConstants()
 {
-    smchandlerRelation(s, pageDbIn, s', pageDbOut) && smchandlerInvariant(s, s')
+    reveal ValidRegState();
+    var entry := s.regs[R0] == KOM_SMC_ENTER || s.regs[R0] == KOM_SMC_RESUME;
+    smchandlerRelation(s, pageDbIn, s', pageDbOut) &&
+        smchandlerInvariant(s, s', entry)
 }
 
 // lemma for allocatePage; FIXME: not trusted, should not be in a .s.dfy file
